examples/tactics/TestBV.fst
@@ -15,7 +15,7 @@ let test3 (x y : uint_t 64) =
 let test4 (x y : uint_t 64) = 
   assert_by_tactic (bv_tac ()) 
   (logand #64 (logand #64 x (logxor #64 x y)) y == logand #64 y (logand #64 x (logxor #64 y x)))
-//canot prove
+//cannot prove
 // let test5 (x : uint_t 32) =
 //   assert_by_tactic (prune "";; addns "Prims";; bv_tac ())
 //     (shift_left #32 x 3 == shift_left #32 (shift_left #32 x 2) 1)
